Definition for cred_fun and prove for soundness of sred_fun

nominal_unification_computable/NU_Computable.thy
@@ -4,8 +4,8 @@ theory NU_Computable
 begin
 (*>*)
 
-definition rank_sred :: "((((trm \<times> trm) list \<times> (char list \<times> trm) list) \<times> substs \<times> bool) \<times>
-      ((trm \<times> trm) list \<times> (char list \<times> trm) list) \<times> substs \<times> bool) set" where
+definition rank_sred :: "((((trm \<times> trm) list \<times> (char list \<times> trm) list) \<times> fresh_envs \<times> substs \<times> bool) \<times>
+      ((trm \<times> trm) list \<times> (char list \<times> trm) list) \<times> fresh_envs \<times> substs \<times> bool) set" where
 "rank_sred =
   measures [
     \<lambda>((eprobs, fprobs), s, B). card (vars_eprobs eprobs),
@@ -14,35 +14,35 @@ definition rank_sred :: "((((trm \<times> trm) list \<times> (char list \<times>
   ]"
 
 
-function (sequential) sred_fun :: "(problem_type \<times> substs \<times> bool) \<Rightarrow> (problem_type \<times> substs \<times> bool)" where
- "sred_fun (((Unit \<approx>? Unit) # xs, ys), s, B) = sred_fun ((xs,ys), s, B)" |
- "sred_fun (((Paar t1 t2 \<approx>? Paar s1 s2)#xs,ys), s, B) = sred_fun (((t1\<approx>?s1)#(t2\<approx>?s2)#xs,ys), s, B)" |
- "sred_fun (((Func F t1 \<approx>? Func G t2)#xs,ys), s, B) = (if F = G then
-                                                        sred_fun(((t1\<approx>?t2)#xs,ys),s, B)         
+function (sequential) sred_fun :: "(problem_type \<times> fresh_envs \<times> substs \<times> bool) \<Rightarrow> (problem_type \<times> fresh_envs \<times> substs \<times> bool)" where
+ "sred_fun (((Unit \<approx>? Unit) # xs, ys), nabla, s, B) = sred_fun ((xs,ys), nabla, s, B)" |
+ "sred_fun (((Paar t1 t2 \<approx>? Paar s1 s2)#xs,ys), nabla, s, B) = sred_fun (((t1\<approx>?s1)#(t2\<approx>?s2)#xs,ys), nabla, s, B)" |
+ "sred_fun (((Func F t1 \<approx>? Func G t2)#xs,ys), nabla, s, B) = (if F = G then
+                                                        sred_fun(((t1\<approx>?t2)#xs,ys), nabla, s, B)         
                                                        else
-                                                        (((Func F t1 \<approx>? Func G t2)#xs,ys), s, False))" |
- "sred_fun (((Abst a t1 \<approx>? Abst b t2)#xs,ys), s, B) = (if a = b then
-                                                        sred_fun (((t1\<approx>?t2)#xs,ys), s, B)
+                                                        (((Func F t1 \<approx>? Func G t2)#xs,ys), nabla, s, False))" |
+ "sred_fun (((Abst a t1 \<approx>? Abst b t2)#xs,ys), nabla, s, B) = (if a = b then
+                                                        sred_fun (((t1\<approx>?t2)#xs,ys), nabla, s, B)
                                                        else
-                                                        sred_fun (((t1\<approx>?swap [(a,b)] t2)#xs,(a\<sharp>?t2)#ys), s, B))"|
- "sred_fun (((Atom a\<approx>?Atom b)#xs,ys), s, B) = (if a = b then
-                                                sred_fun ((xs,ys), s, B)
+                                                        sred_fun (((t1\<approx>?swap [(a,b)] t2)#xs,(a\<sharp>?t2)#ys), nabla, s, B))"|
+ "sred_fun (((Atom a\<approx>?Atom b)#xs,ys), nabla, s, B) = (if a = b then
+                                                sred_fun ((xs,ys), nabla, s, B)
                                                else
-                                                (((Atom a \<approx>? Atom b)#xs,ys), s, False))" |
- "sred_fun (((Susp pi1 X\<approx>?Susp pi2 Y)#xs,ys), s, B) = (if X =Y then 
-                                                        sred_fun ((xs,(map (\<lambda>a. a\<sharp>? Susp [] X) (ds_list pi1 pi2))@ys), s, B)
+                                                (((Atom a \<approx>? Atom b)#xs,ys), nabla, s, False))" |
+ "sred_fun (((Susp pi1 X\<approx>?Susp pi2 Y)#xs,ys), nabla, s, B) = (if X =Y then 
+                                                        sred_fun ((xs,(map (\<lambda>a. a\<sharp>? Susp [] X) (ds_list pi1 pi2))@ys), nabla, s, B)
                                                        else
-                                                        sred_fun (apply_subst [(X,swap (rev pi1) (Susp pi2 Y))] (xs,ys), [(X,swap (rev pi1) (Susp pi2 Y))] \<bullet> s, B))"|
- "sred_fun (((Susp pi X\<approx>?t)#xs,ys), s, B) = (if \<not> (occurs X t) then
-                                              sred_fun (apply_subst [(X,swap (rev pi) t)] (xs,ys), [(X,swap (rev pi) t)] \<bullet> s, B)
+                                                        sred_fun (apply_subst [(X,swap (rev pi1) (Susp pi2 Y))] (xs,ys), nabla, [(X,swap (rev pi1) (Susp pi2 Y))] \<bullet> s, B))"|
+ "sred_fun (((Susp pi X\<approx>?t)#xs,ys), nabla, s, B) = (if \<not> (occurs X t) then
+                                              sred_fun (apply_subst [(X,swap (rev pi) t)] (xs,ys), nabla, [(X,swap (rev pi) t)] \<bullet> s, B)
                                              else
-                                              (((Susp pi X\<approx>?t)#xs,ys), s, False))" |
- "sred_fun (((t\<approx>?Susp pi X)#xs,ys), s, B) = (if \<not> (occurs X t) then
-                                              sred_fun (apply_subst [(X,swap (rev pi) t)] (xs,ys), [(X,swap (rev pi) t)] \<bullet> s, B)
+                                              (((Susp pi X\<approx>?t)#xs,ys), nabla, s, False))" |
+ "sred_fun (((t\<approx>?Susp pi X)#xs,ys), nabla, s, B) = (if \<not> (occurs X t) then
+                                              sred_fun (apply_subst [(X,swap (rev pi) t)] (xs,ys), nabla, [(X,swap (rev pi) t)] \<bullet> s, B)
                                              else
-                                              (((t\<approx>?Susp pi X)#xs,ys), s, False))" |
- "sred_fun (([],ys), s, B) = (([], ys), s, B)" |
- "sred_fun ((e#xs, ys), s, B) = ((e#xs, ys), s, False)" 
+                                              (((t\<approx>?Susp pi X)#xs,ys), nabla, s, False))" |
+ "sred_fun (([],ys), nabla, s, B) = (([], ys), nabla, s, B)" |
+ "sred_fun ((e#xs, ys), nabla, s, B) = ((e#xs, ys), nabla, s, False)" 
   by pat_completeness auto
 
 
@@ -52,56 +52,56 @@ proof(relation rank_sred)
   show "wf rank_sred" 
     unfolding rank_sred_def by simp
 
-  show "\<And>xs ys s B. (((xs, ys), s, B), ((Unit, Unit) # xs, ys), s, B) \<in> rank_sred"
+  show "\<And>xs ys nabla s B. (((xs, ys), nabla, s, B), ((Unit, Unit) # xs, ys), nabla, s, B) \<in> rank_sred"
     unfolding rank_sred_def by simp
 
-  show "\<And>t1 t2 s1 s2 xs ys s B.
-       ((((t1, s1) # (t2, s2) # xs, ys), s, B), ((Paar t1 t2, Paar s1 s2) # xs, ys), s, B) \<in> rank_sred"
+  show "\<And>t1 t2 s1 s2 xs ys nabla s B.
+       ((((t1, s1) # (t2, s2) # xs, ys), nabla, s, B), ((Paar t1 t2, Paar s1 s2) # xs, ys), nabla, s, B) \<in> rank_sred"
     unfolding rank_sred_def vars_eprobs.simps size_eprobs.simps size_trm.simps vars_trm.simps
     by (simp add: Un_commute Un_left_commute)
 
-  show "\<And>t1 F G t2 xs ys s B. F = G \<Longrightarrow>
-       ((((t1, t2) # xs, ys), s, B), ((trm.Func F t1, trm.Func G t2) # xs, ys), s, B)
+  show "\<And>t1 F G t2 xs ys nabla s B. F = G \<Longrightarrow>
+       ((((t1, t2) # xs, ys), nabla, s, B), ((trm.Func F t1, trm.Func G t2) # xs, ys), nabla, s, B)
        \<in> rank_sred"
     unfolding rank_sred_def vars_eprobs.simps size_eprobs.simps size_trm.simps vars_trm.simps
     by simp
 
-  show  "\<And>a t1 b t2 xs ys s B. a = b \<Longrightarrow>
-       ((((t1, t2) # xs, ys), s, B), ((Abst a t1, Abst b t2) # xs, ys), s, B) \<in> rank_sred"
+  show  "\<And>a t1 b t2 xs ys nabla s B. a = b \<Longrightarrow>
+       ((((t1, t2) # xs, ys), nabla, s, B), ((Abst a t1, Abst b t2) # xs, ys), nabla, s, B) \<in> rank_sred"
     unfolding rank_sred_def vars_eprobs.simps 
       size_eprobs.simps size_trm.simps vars_trm.simps
     by simp
 
-  show "\<And>a t1 b t2 xs ys s B.
+  show "\<And>a t1 b t2 xs ys nabla s B.
        a \<noteq> b \<Longrightarrow>
-       ((((t1, swap [(a, b)] t2) # xs, (a, t2) # ys), s, B), ((Abst a t1, Abst b t2) # xs, ys),
-        s, B)
+       ((((t1, swap [(a, b)] t2) # xs, (a, t2) # ys), nabla, s, B), ((Abst a t1, Abst b t2) # xs, ys),
+        nabla, s, B)
        \<in> rank_sred"
     using vars_swap unfolding rank_sred_def vars_eprobs.simps 
         size_eprobs.simps size_trm.simps vars_trm.simps
     by simp
 
-  show "\<And>a b xs ys s B. a = b \<Longrightarrow>
-  (((xs, ys), s, B), ((Atom a, Atom b) # xs, ys), s, B) \<in> rank_sred"
+  show "\<And>a b xs ys nabla s B. a = b \<Longrightarrow>
+  (((xs, ys), nabla, s, B), ((Atom a, Atom b) # xs, ys), nabla, s, B) \<in> rank_sred"
     unfolding rank_sred_def vars_eprobs.simps 
       size_eprobs.simps size_trm.simps vars_trm.simps 
     by simp
 
-  show "\<And>pi1 X pi2 Y xs ys s B.
+  show "\<And>pi1 X pi2 Y xs ys nabla s B.
        X = Y \<Longrightarrow>
-       (((xs, map (\<lambda>a. (a, Susp [] X)) (ds_list pi1 pi2) @ ys), s, B),
-        ((Susp pi1 X, Susp pi2 Y) # xs, ys), s, B)
+       (((xs, map (\<lambda>a. (a, Susp [] X)) (ds_list pi1 pi2) @ ys), nabla, s, B),
+        ((Susp pi1 X, Susp pi2 Y) # xs, ys), nabla, s, B)
        \<in> rank_sred"
   proof-
-    fix pi1 pi2 xs ys s B and X Y :: string
+    fix pi1 pi2 xs ys nabla s B and X Y :: string
     assume "X = Y"
     hence vars: "vars_eprobs ((Susp pi1 X, Susp pi2 Y) # xs) = {X} \<union> vars_eprobs xs" and
           size: "size_eprobs ((Susp pi1 X, Susp pi2 Y) # xs) = 2 + size_eprobs xs"
       unfolding vars_eprobs.simps size_eprobs.simps by simp+
     have size_leq: "size_eprobs xs < size_eprobs ((Susp pi1 Y, Susp pi2 Y) # xs)"
       by simp
-    have "(((xs, map (\<lambda>a. (a, Susp [] X)) (ds_list pi1 pi2) @ ys), s, B),
-        ((Susp pi1 X, Susp pi2 Y) # xs, ys), s, B)
+    have "(((xs, map (\<lambda>a. (a, Susp [] X)) (ds_list pi1 pi2) @ ys), nabla, s, B),
+        ((Susp pi1 X, Susp pi2 Y) # xs, ys), nabla, s, B)
        \<in> rank_sred"
     proof(cases "X \<in> vars_eprobs xs")
       case True
@@ -116,15 +116,15 @@ proof(relation rank_sred)
       then show ?thesis 
         using \<open>X = Y\<close> unfolding rank_sred_def by simp
     qed
-    thus "(((xs, map (\<lambda>a. (a, Susp [] X)) (ds_list pi1 pi2) @ ys), s, B),
-        ((Susp pi1 X, Susp pi2 Y) # xs, ys), s, B)
+    thus "(((xs, map (\<lambda>a. (a, Susp [] X)) (ds_list pi1 pi2) @ ys), nabla, s, B),
+        ((Susp pi1 X, Susp pi2 Y) # xs, ys), nabla, s, B)
        \<in> rank_sred" by simp
   qed
 
-  have aux1: "\<not> occurs X t \<Longrightarrow> ((apply_subst [(X, swap (rev pi) t)] (xs, ys),
+  have aux1: "\<not> occurs X t \<Longrightarrow> ((apply_subst [(X, swap (rev pi) t)] (xs, ys), nabla,
          [(X, swap (rev pi) t)] \<bullet> s, B),
-        ((Susp pi X, t) # xs, ys), s, B)
-       \<in> rank_sred" for X t pi xs ys s B
+        ((Susp pi X, t) # xs, ys), nabla, s, B)
+       \<in> rank_sred" for X t pi xs ys nabla s B
   proof-
     let ?union = "insert X (vars_trm t \<union> vars_eprobs xs)"
       and ?size = "size_trm t + size_eprobs xs"
@@ -141,10 +141,10 @@ proof(relation rank_sred)
       using vars_decrease[OF assm] unfolding rank_sred_def by simp
   qed
 
-  have aux2: "\<not> occurs X t \<Longrightarrow> ((apply_subst [(X, swap (rev pi) t)] (xs, ys),
+  have aux2: "\<not> occurs X t \<Longrightarrow> ((apply_subst [(X, swap (rev pi) t)] (xs, ys), nabla,
          [(X, swap (rev pi) t)] \<bullet> s, B),
-        ((t, Susp pi X) # xs, ys), s, B)
-       \<in> rank_sred" for X t pi xs ys s B
+        ((t, Susp pi X) # xs, ys), nabla, s, B)
+       \<in> rank_sred" for X t pi xs ys nabla s B
   proof-
     let ?union = "insert X (vars_trm t \<union> vars_eprobs xs)"
       and ?size = "size_trm t + size_eprobs xs"
@@ -161,112 +161,508 @@ proof(relation rank_sred)
       using vars_decrease[OF assm] unfolding rank_sred_def by simp
   qed
 
-  show "\<And>pi1 X pi2 Y xs ys s B.
+  show "\<And>pi1 X pi2 Y xs ys nabla s B.
        X \<noteq> Y \<Longrightarrow>
-       ((apply_subst [(X, swap (rev pi1) (Susp pi2 Y))] (xs, ys),
+       ((apply_subst [(X, swap (rev pi1) (Susp pi2 Y))] (xs, ys), nabla,
          [(X, swap (rev pi1) (Susp pi2 Y))] \<bullet> s, B),
-        ((Susp pi1 X, Susp pi2 Y) # xs, ys), s, B)
+        ((Susp pi1 X, Susp pi2 Y) # xs, ys), nabla, s, B)
        \<in> rank_sred"
   proof-
-    fix X Y :: string and pi1 pi2 xs ys s B
+    fix X Y :: string and pi1 pi2 xs ys nabla s B
     assume "X \<noteq> Y"
     hence not_occurs: "\<not> occurs X (Susp pi2 Y)" 
       unfolding occurs.simps by simp
     thus "X \<noteq> Y \<Longrightarrow>
         X \<noteq> Y \<Longrightarrow>
-       ((apply_subst [(X, swap (rev pi1) (Susp pi2 Y))] (xs, ys),
+       ((apply_subst [(X, swap (rev pi1) (Susp pi2 Y))] (xs, ys), nabla,
          [(X, swap (rev pi1) (Susp pi2 Y))] \<bullet> s, B),
-        ((Susp pi1 X, Susp pi2 Y) # xs, ys), s, B)
+        ((Susp pi1 X, Susp pi2 Y) # xs, ys), nabla, s, B)
        \<in> rank_sred" 
        using aux1[OF not_occurs] unfolding rank_sred_def by simp
    qed
 
-   show "\<And>pi X v va xs ys s B.
+   show "\<And>pi X v va xs ys nabla s B.
        \<not> occurs X (Abst v va) \<Longrightarrow>
-       ((apply_subst [(X, swap (rev pi) (Abst v va))] (xs, ys),
+       ((apply_subst [(X, swap (rev pi) (Abst v va))] (xs, ys), nabla,
          [(X, swap (rev pi) (Abst v va))] \<bullet> s, B),
-        ((Susp pi X, Abst v va) # xs, ys), s, B)
+        ((Susp pi X, Abst v va) # xs, ys), nabla, s, B)
        \<in> rank_sred"
      using aux1 by blast
 
-   show "\<And>pi X xs ys s B.
+   show "\<And>pi X xs ys nabla s B.
        \<not> occurs X Unit \<Longrightarrow>
-       ((apply_subst [(X, swap (rev pi) Unit)] (xs, ys), [(X, swap (rev pi) Unit)] \<bullet> s, B),
-        ((Susp pi X, Unit) # xs, ys), s, B)
+       ((apply_subst [(X, swap (rev pi) Unit)] (xs, ys), nabla, [(X, swap (rev pi) Unit)] \<bullet> s, B),
+        ((Susp pi X, Unit) # xs, ys), nabla, s, B)
        \<in> rank_sred" using aux1 by blast
 
-   show "\<And>pi X v xs ys s B.
+   show "\<And>pi X v xs ys nabla s B.
        \<not> occurs X (Atom v) \<Longrightarrow>
-       ((apply_subst [(X, swap (rev pi) (Atom v))] (xs, ys), [(X, swap (rev pi) (Atom v))] \<bullet> s,
+       ((apply_subst [(X, swap (rev pi) (Atom v))] (xs, ys), nabla, [(X, swap (rev pi) (Atom v))] \<bullet> s,
          B),
-        ((Susp pi X, Atom v) # xs, ys), s, B)
+        ((Susp pi X, Atom v) # xs, ys), nabla, s, B)
        \<in> rank_sred" using aux1 by blast
 
-   show "\<And>pi X v va xs ys s B.
+   show "\<And>pi X v va xs ys nabla s B.
        \<not> occurs X (Paar v va) \<Longrightarrow>
-       ((apply_subst [(X, swap (rev pi) (Paar v va))] (xs, ys),
+       ((apply_subst [(X, swap (rev pi) (Paar v va))] (xs, ys), nabla,
          [(X, swap (rev pi) (Paar v va))] \<bullet> s, B),
-        ((Susp pi X, Paar v va) # xs, ys), s, B)
+        ((Susp pi X, Paar v va) # xs, ys), nabla, s, B)
        \<in> rank_sred" using aux1 by blast
 
-   show "\<And>pi X v va xs ys s B.
+   show "\<And>pi X v va xs ys nabla s B.
        \<not> occurs X (trm.Func v va) \<Longrightarrow>
-       ((apply_subst [(X, swap (rev pi) (trm.Func v va))] (xs, ys),
+       ((apply_subst [(X, swap (rev pi) (trm.Func v va))] (xs, ys), nabla,
          [(X, swap (rev pi) (trm.Func v va))] \<bullet> s, B),
-        ((Susp pi X, trm.Func v va) # xs, ys), s, B)
+        ((Susp pi X, trm.Func v va) # xs, ys), nabla, s, B)
        \<in> rank_sred" using aux1 by blast
 
-   show "\<And>v va pi X xs ys s B.
+   show "\<And>v va pi X xs ys nabla s B.
        \<not> occurs X (Abst v va) \<Longrightarrow>
-       ((apply_subst [(X, swap (rev pi) (Abst v va))] (xs, ys),
+       ((apply_subst [(X, swap (rev pi) (Abst v va))] (xs, ys), nabla,
          [(X, swap (rev pi) (Abst v va))] \<bullet> s, B),
-        ((Abst v va, Susp pi X) # xs, ys), s, B)
+        ((Abst v va, Susp pi X) # xs, ys), nabla, s, B)
        \<in> rank_sred" using aux2 by blast
 
-   show "\<And>pi X xs ys s B.
+   show "\<And>pi X xs ys nabla s B.
        \<not> occurs X Unit \<Longrightarrow>
-       ((apply_subst [(X, swap (rev pi) Unit)] (xs, ys), [(X, swap (rev pi) Unit)] \<bullet> s, B),
-        ((Unit, Susp pi X) # xs, ys), s, B)
-       \<in> rank_sred" using aux2 by blast
-
-   show "\<And>v pi X xs ys s B.
-       \<not> occurs X (Atom v) \<Longrightarrow>
-       ((apply_subst [(X, swap (rev pi) (Atom v))] (xs, ys), [(X, swap (rev pi) (Atom v))] \<bullet> s,
+       ((apply_subst [(X, swap (rev pi) Unit)] (xs, ys), nabla, [(X, swap (rev pi) Unit)] \<bullet> s,
          B),
-        ((Atom v, Susp pi X) # xs, ys), s, B)
+        ((Unit, Susp pi X) # xs, ys), nabla, s, B)
        \<in> rank_sred" using aux2 by blast
 
-   show "\<And>v va pi X xs ys s B.
+   show "\<And>v pi X xs ys nabla s B.
+       \<not> occurs X (Atom v) \<Longrightarrow>
+       ((apply_subst [(X, swap (rev pi) (Atom v))] (xs, ys), nabla,
+         [(X, swap (rev pi) (Atom v))] \<bullet> s, B),
+        ((Atom v, Susp pi X) # xs, ys), nabla, s, B)
+       \<in> rank_sred" using aux2 by blast
+
+   show "\<And>v va pi X xs ys nabla s B.
        \<not> occurs X (Paar v va) \<Longrightarrow>
-       ((apply_subst [(X, swap (rev pi) (Paar v va))] (xs, ys),
+       ((apply_subst [(X, swap (rev pi) (Paar v va))] (xs, ys), nabla,
          [(X, swap (rev pi) (Paar v va))] \<bullet> s, B),
-        ((Paar v va, Susp pi X) # xs, ys), s, B)
+        ((Paar v va, Susp pi X) # xs, ys), nabla, s, B)
        \<in> rank_sred" using aux2 by blast
 
-   show "\<And>v va pi X xs ys s B.
+   show "\<And>v va pi X xs ys nabla s B.
        \<not> occurs X (trm.Func v va) \<Longrightarrow>
-       ((apply_subst [(X, swap (rev pi) (trm.Func v va))] (xs, ys),
+       ((apply_subst [(X, swap (rev pi) (trm.Func v va))] (xs, ys), nabla,
          [(X, swap (rev pi) (trm.Func v va))] \<bullet> s, B),
-        ((trm.Func v va, Susp pi X) # xs, ys), s, B)
+        ((trm.Func v va, Susp pi X) # xs, ys), nabla, s, B)
        \<in> rank_sred" using aux2 by blast
+ qed
+
+lemma if_sred_then_not_equal:
+  assumes "P1 \<turnstile> s \<leadsto> P2"
+  shows "P1 \<noteq> P2"
+  using assms
+proof(cases rule: s_red.cases)
+  case (var_1_sred X t pi xs ys)
+  then show ?thesis 
+    by (metis assms not_Cons_self2 sred_rtc.simps sred_rtc_no_cycle subst_id_left)
+next
+  case (var_2_sred X t pi xs ys)
+  then show ?thesis 
+    by (metis assms not_Cons_self2 sred_rtc.simps sred_rtc_no_cycle subst_id_left)
+qed (simp_all)
+
+
+lemma sred_fun_sound:
+  assumes  "sred_fun (P1, nabla, s, True) = (P2, nabla', s', B)"
+  shows "\<exists> s1. P1 \<turnstile> s1 \<leadsto>\<^sup>* P2"
+  using assms
+proof(induction "(P1, nabla, s, True)" arbitrary: P1 nabla s rule: sred_fun.induct)
+  case (1 xs ys nabla s)
+  hence fun_step:
+    "sred_fun ((xs, ys), nabla, s, True) = (P2, nabla', s', B)"
+    by simp
+  with 1(1) show "\<exists>s1. ((Unit, Unit) # xs, ys) \<turnstile> s1 \<leadsto>\<^sup>* P2" 
+    by auto
+next
+  case (2 t1 t2 s1 s2 xs ys nabla s)
+  hence fun_step:
+    "sred_fun (((t1, s1) # (t2, s2) # xs, ys), nabla, s, True) = (P2, nabla', s', B)"
+    by simp
+   with 2(1) show "\<exists>\<sigma>. ((Paar t1 t2, Paar s1 s2) # xs, ys) \<turnstile> \<sigma> \<leadsto>\<^sup>* P2" 
+     by auto
+next
+  case (3 F t1 G t2 xs ys nabla s)
+  then show "\<exists>s1. ((Func F t1, Func G t2) # xs, ys) \<turnstile> s1 \<leadsto>\<^sup>* P2"
+  proof(cases "F = G")
+    case True
+    with 3(2) have "sred_fun (((t1, t2) # xs, ys), nabla, s, True) = (P2, nabla', s', B)"
+      by simp
+    with 3(1) True
+    show "\<exists>s1. ((Func F t1, Func G t2) # xs, ys) \<turnstile> s1 \<leadsto>\<^sup>* P2"
+      by auto
+  next
+    case False
+    hence "sred_fun (((Func F t1, Func G t2) # xs, ys), nabla, s, True) 
+    = (((Func F t1 \<approx>? Func G t2)#xs,ys), nabla, s, False)" 
+      by simp
+    with 3(2) have P2_def: "P2 = ((Func F t1 \<approx>? Func G t2)#xs,ys)" 
+      by simp
+    have "((Func F t1, Func G t2) # xs, ys) \<turnstile> [] \<leadsto>\<^sup>* P2"
+      using P2_def sred_refl by simp
+    thus "\<exists>s1. ((Func F t1, Func G t2) # xs, ys) \<turnstile> s1 \<leadsto>\<^sup>* P2" 
+      by auto
+  qed
+next
+  case (4 a t1 b t2 xs ys nabla s)
+  then show "\<exists>s1. ((Abst a t1, Abst b t2) # xs, ys) \<turnstile> s1 \<leadsto>\<^sup>* P2" 
+  proof(cases "a = b")
+    case True
+    with 4(3) have "sred_fun (((t1, t2) # xs, ys), nabla, s, True) = (P2, nabla', s', B)"
+      by simp
+    with 4(1) True
+    show "\<exists>s1. ((Abst a t1, Abst b t2) # xs, ys) \<turnstile> s1 \<leadsto>\<^sup>* P2"
+      by auto
+  next
+    case False
+    with 4(3) have "sred_fun (((t1, swap [(a, b)] t2) # xs, (a, t2) # ys), nabla, s, True) =
+    (P2, nabla', s', B)" by simp
+    with 4(2) False
+    show "\<exists>s1. ((Abst a t1, Abst b t2) # xs, ys) \<turnstile> s1 \<leadsto>\<^sup>* P2"
+      by auto
+  qed
+next
+  case (5 a b xs ys nabla s)
+  then show "\<exists>s1. ((Atom a, Atom b) # xs, ys) \<turnstile> s1 \<leadsto>\<^sup>* P2"
+  proof(cases "a=b")
+    case True
+    with 5(2) have "sred_fun ((xs, ys), nabla, s, True) = (P2, nabla', s', B)"
+      by simp
+    with 5(1) True show "\<exists>s1. ((Atom a, Atom b) # xs, ys) \<turnstile> s1 \<leadsto>\<^sup>* P2"
+      by auto
+  next
+    case False
+    hence "sred_fun (((Atom a, Atom b) # xs, ys), nabla, s, True) 
+    = (((Atom a \<approx>? Atom b)#xs,ys), nabla, s, False)" 
+      by simp
+    with 5(2) have "P2 = ((Atom a \<approx>? Atom b)#xs,ys)" 
+      by simp
+    hence "((Atom a, Atom b) # xs, ys) \<turnstile> [] \<leadsto>\<^sup>* P2"
+      using sred_refl by simp
+    then show "\<exists>s1. ((Atom a, Atom b) # xs, ys) \<turnstile> s1 \<leadsto>\<^sup>* P2"
+      by auto
+  qed
+next
+  case (6 pi1 X pi2 Y xs ys nabla s)
+  then show "\<exists>s1. ((Susp pi1 X, Susp pi2 Y) # xs, ys) \<turnstile> s1 \<leadsto>\<^sup>* P2"
+  proof(cases "X = Y")
+    case True
+    with 6(3) have "sred_fun ((xs, map (\<lambda>a. (a, Susp [] X)) (ds_list pi1 pi2) @ ys), nabla, s, True) =
+    (P2, nabla', s', B)"
+      by simp
+    with 6(1) True show "\<exists>s1. ((Susp pi1 X, Susp pi2 Y) # xs, ys) \<turnstile> s1 \<leadsto>\<^sup>* P2"
+      by auto
+  next
+    case False
+    with 6(3) have "sred_fun
+     (apply_subst [(X, swap (rev pi1) (Susp pi2 Y))] (xs, ys), nabla,
+      [(X, swap (rev pi1) (Susp pi2 Y))] \<bullet> s, True) =
+    (P2, nabla', s', B)" by simp
+    with 6(2) False obtain s2 where 
+      more: "apply_subst [(X, swap (rev pi1) (Susp pi2 Y))] (xs, ys) \<turnstile> s2 \<leadsto>\<^sup>* P2"
+      by auto
+    moreover have first: "((Susp pi1 X, Susp pi2 Y) # xs, ys) \<turnstile> [(X, swap (rev pi1) (Susp pi2 Y))]
+                                       \<leadsto> apply_subst [(X, swap (rev pi1) (Susp pi2 Y))] (xs, ys)"
+      using False var_1_sred occurs.simps by force
+    ultimately have 
+      "((Susp pi1 X, Susp pi2 Y) # xs, ys) \<turnstile> s2 \<bullet> [(X, swap (rev pi1) (Susp pi2 Y))] \<leadsto>\<^sup>* P2"
+      using sred_rtc_step by simp
+    then show "\<exists>s1. ((Susp pi1 X, Susp pi2 Y) # xs, ys) \<turnstile> s1 \<leadsto>\<^sup>* P2"
+      by auto
+  qed
+next
+  case ("7_1" pi X a t xs ys nabla s)
+  then show "\<exists>s1. ((Susp pi X, Abst a t) # xs, ys) \<turnstile> s1 \<leadsto>\<^sup>* P2"
+  proof(cases "occurs X (Abst a t)")
+    case True
+    hence "sred_fun (((Susp pi X, Abst a t) # xs, ys), nabla, s, True) 
+      = (((Susp pi X, Abst a t) # xs, ys), nabla, s, False)" by simp
+    with "7_1"(2) have "((Susp pi X, Abst a t) # xs, ys) \<turnstile> [] \<leadsto>\<^sup>* P2" 
+      by auto
+    then show "\<exists>s1. ((Susp pi X, Abst a t) # xs, ys) \<turnstile> s1 \<leadsto>\<^sup>* P2" 
+      by auto
+  next
+    case False
+    with "7_1"(2) have "sred_fun
+     (apply_subst [(X, swap (rev pi) (Abst a t))] (xs, ys), nabla,
+      [(X, swap (rev pi) (Abst a t))] \<bullet> s, True) =
+    (P2, nabla', s', B)" by simp
+    with "7_1"(1) False obtain s2 where
+    more: "apply_subst [(X, swap (rev pi) (Abst a t))] (xs, ys) \<turnstile> s2 \<leadsto>\<^sup>* P2"
+      by auto
+    moreover have first: "((Susp pi X, Abst a t) # xs, ys) \<turnstile> 
+        [(X, swap (rev pi) (Abst a t))] \<leadsto> apply_subst [(X, swap (rev pi) (Abst a t))] (xs, ys)"
+      using False var_1_sred occurs.simps by force
+    ultimately have "((Susp pi X, Abst a t) # xs, ys) \<turnstile> 
+              s2 \<bullet> [(X, swap (rev pi) (Abst a t))] \<leadsto>\<^sup>* P2"
+      using sred_rtc_step by simp
+    then show "\<exists>s1. ((Susp pi X, Abst a t) # xs, ys) \<turnstile> s1 \<leadsto>\<^sup>* P2" 
+      by auto
+  qed
+next
+  case ("7_2" pi X xs ys nabla s)
+  hence "sred_fun
+     (apply_subst [(X, swap (rev pi) Unit)] (xs, ys), nabla, [(X, swap (rev pi) Unit)] \<bullet> s,
+      True) =
+    (P2, nabla', s', B)" by simp
+  moreover have not_occurs: "\<not> occurs X Unit" by simp
+  ultimately obtain s2 where
+    more: "apply_subst [(X, swap (rev pi) Unit)] (xs, ys) \<turnstile> s2 \<leadsto>\<^sup>* P2"
+    using "7_2"(1) by auto
+  moreover have first: "((Susp pi X, Unit) # xs, ys) \<turnstile> [(X, swap (rev pi) Unit)]
+      \<leadsto> apply_subst [(X, swap (rev pi) Unit)] (xs, ys)"
+    using not_occurs var_1_sred by blast
+  ultimately have "((Susp pi X, Unit) # xs, ys) \<turnstile> s2 \<bullet> [(X, swap (rev pi) Unit)] \<leadsto>\<^sup>* P2"
+    using sred_rtc_step by simp
+  then show "\<exists>s1. ((Susp pi X, Unit) # xs, ys) \<turnstile> s1 \<leadsto>\<^sup>* P2" 
+    by auto
+next
+  case ("7_3" pi X a xs ys nabla s)
+  hence "sred_fun
+     (apply_subst [(X, swap (rev pi) (Atom a))] (xs, ys), nabla, [(X, swap (rev pi) (Atom a))] \<bullet> s,
+      True) =
+    (P2, nabla', s', B)" by simp
+  moreover have not_occurs: "\<not> occurs X (Atom a)" by simp
+  ultimately obtain s2 where
+    more: "apply_subst [(X, swap (rev pi) (Atom a))] (xs, ys) \<turnstile> s2 \<leadsto>\<^sup>* P2"
+    using "7_3"(1) by auto
+  moreover have first: "((Susp pi X, Atom a) # xs, ys) \<turnstile> [(X, swap (rev pi) (Atom a))]
+      \<leadsto> apply_subst [(X, swap (rev pi) (Atom a))] (xs, ys)"
+    using not_occurs var_1_sred by blast
+  ultimately have "((Susp pi X, Atom a) # xs, ys) \<turnstile> s2 \<bullet> [(X, swap (rev pi) (Atom a))] \<leadsto>\<^sup>* P2"
+    using sred_rtc_step by simp
+  then show "\<exists>s1. ((Susp pi X, Atom a) # xs, ys) \<turnstile> s1 \<leadsto>\<^sup>* P2" 
+    by auto
+next
+  case ("7_4" pi X t1 t2 xs ys nabla s)
+  then show "\<exists>s1. ((Susp pi X, Paar t1 t2) # xs, ys) \<turnstile> s1 \<leadsto>\<^sup>* P2"
+  proof(cases "occurs X (Paar t1 t2)")
+    case True
+    hence "sred_fun (((Susp pi X, Paar t1 t2) # xs, ys), nabla, s, True) 
+      = (((Susp pi X, Paar t1 t2) # xs, ys), nabla, s, False)" by simp
+    with "7_4"(2) have "((Susp pi X, Paar t1 t2) # xs, ys) \<turnstile> [] \<leadsto>\<^sup>* P2" 
+      by auto
+    then show "\<exists>s1. ((Susp pi X, Paar t1 t2) # xs, ys) \<turnstile> s1 \<leadsto>\<^sup>* P2" 
+      by auto
+  next
+    case False
+    with "7_4"(2) have "sred_fun
+     (apply_subst [(X, swap (rev pi) (Paar t1 t2))] (xs, ys), nabla,
+      [(X, swap (rev pi) (Paar t1 t2))] \<bullet> s, True) =
+    (P2, nabla', s', B)" by simp
+    with "7_4"(1) False obtain s2 where
+    more: "apply_subst [(X, swap (rev pi) (Paar t1 t2))] (xs, ys) \<turnstile> s2 \<leadsto>\<^sup>* P2"
+      by auto
+    moreover have first: "((Susp pi X, Paar t1 t2) # xs, ys) \<turnstile> 
+        [(X, swap (rev pi) (Paar t1 t2))] \<leadsto> apply_subst [(X, swap (rev pi) (Paar t1 t2))] (xs, ys)"
+      using False var_1_sred occurs.simps by force
+    ultimately have "((Susp pi X, Paar t1 t2) # xs, ys) \<turnstile> 
+              s2 \<bullet> [(X, swap (rev pi) (Paar t1 t2))] \<leadsto>\<^sup>* P2"
+      using sred_rtc_step by simp
+    then show "\<exists>s1. ((Susp pi X, Paar t1 t2) # xs, ys) \<turnstile> s1 \<leadsto>\<^sup>* P2" 
+      by auto
+  qed
+next
+  case ("7_5" pi X F t xs ys nabla s)
+  then show "\<exists>s1. ((Susp pi X, Func F t) # xs, ys) \<turnstile> s1 \<leadsto>\<^sup>* P2"
+  proof(cases "occurs X (Func F t)")
+    case True
+    hence "sred_fun (((Susp pi X, Func F t) # xs, ys), nabla, s, True) 
+      = (((Susp pi X, Func F t) # xs, ys), nabla, s, False)" by simp
+    with "7_5"(2) have "((Susp pi X, Func F t) # xs, ys) \<turnstile> [] \<leadsto>\<^sup>* P2" 
+      by auto
+    then show "\<exists>s1. ((Susp pi X, Func F t) # xs, ys) \<turnstile> s1 \<leadsto>\<^sup>* P2" 
+      by auto
+  next
+    case False
+    with "7_5"(2) have "sred_fun
+     (apply_subst [(X, swap (rev pi) (Func F t))] (xs, ys), nabla,
+      [(X, swap (rev pi) (Func F t))] \<bullet> s, True) =
+    (P2, nabla', s', B)" by simp
+    with "7_5"(1) False obtain s2 where
+    more: "apply_subst [(X, swap (rev pi) (Func F t))] (xs, ys) \<turnstile> s2 \<leadsto>\<^sup>* P2"
+      by auto
+    moreover have first: "((Susp pi X, Func F t) # xs, ys) \<turnstile> 
+        [(X, swap (rev pi) (Func F t))] \<leadsto> apply_subst [(X, swap (rev pi) (Func F t))] (xs, ys)"
+      using False var_1_sred occurs.simps by force
+    ultimately have "((Susp pi X, Func F t) # xs, ys) \<turnstile> 
+              s2 \<bullet> [(X, swap (rev pi) (Func F t))] \<leadsto>\<^sup>* P2"
+      using sred_rtc_step by simp
+    then show "\<exists>s1. ((Susp pi X, Func F t) # xs, ys) \<turnstile> s1 \<leadsto>\<^sup>* P2" 
+      by auto
+  qed
+next
+  case ("8_1" a t pi X xs ys nabla s)
+   then show "\<exists>s1. ((Abst a t, Susp pi X) # xs, ys) \<turnstile> s1 \<leadsto>\<^sup>* P2"
+  proof(cases "occurs X (Abst a t)")
+    case True
+    hence "sred_fun (((Abst a t, Susp pi X) # xs, ys), nabla, s, True) 
+      = (((Abst a t, Susp pi X) # xs, ys), nabla, s, False)" by simp
+    with "8_1"(2) have "((Abst a t, Susp pi X) # xs, ys) \<turnstile> [] \<leadsto>\<^sup>* P2" 
+      by auto
+    then show "\<exists>s1. ((Abst a t, Susp pi X) # xs, ys) \<turnstile> s1 \<leadsto>\<^sup>* P2" 
+      by auto
+  next
+    case False
+    with "8_1"(2) have "sred_fun
+     (apply_subst [(X, swap (rev pi) (Abst a t))] (xs, ys), nabla,
+      [(X, swap (rev pi) (Abst a t))] \<bullet> s, True) =
+    (P2, nabla', s', B)" by simp
+    with "8_1"(1) False obtain s2 where
+    more: "apply_subst [(X, swap (rev pi) (Abst a t))] (xs, ys) \<turnstile> s2 \<leadsto>\<^sup>* P2"
+      by auto
+    moreover have first: "((Abst a t, Susp pi X) # xs, ys) \<turnstile> 
+        [(X, swap (rev pi) (Abst a t))] \<leadsto> apply_subst [(X, swap (rev pi) (Abst a t))] (xs, ys)"
+      using False var_2_sred occurs.simps by force
+    ultimately have "((Abst a t, Susp pi X) # xs, ys) \<turnstile> 
+              s2 \<bullet> [(X, swap (rev pi) (Abst a t))] \<leadsto>\<^sup>* P2"
+      using sred_rtc_step by simp
+    then show "\<exists>s1. ((Abst a t, Susp pi X) # xs, ys) \<turnstile> s1 \<leadsto>\<^sup>* P2" 
+      by auto
+  qed
+next
+  case ("8_2" pi X xs ys nabla s)
+  hence "sred_fun
+     (apply_subst [(X, swap (rev pi) Unit)] (xs, ys), nabla, [(X, swap (rev pi) Unit)] \<bullet> s,
+      True) =
+    (P2, nabla', s', B)" by simp
+  moreover have not_occurs: "\<not> occurs X Unit" by simp
+  ultimately obtain s2 where
+    more: "apply_subst [(X, swap (rev pi) Unit)] (xs, ys) \<turnstile> s2 \<leadsto>\<^sup>* P2"
+    using "8_2"(1) by auto
+  moreover have first: "((Unit, Susp pi X) # xs, ys) \<turnstile> [(X, swap (rev pi) Unit)]
+      \<leadsto> apply_subst [(X, swap (rev pi) Unit)] (xs, ys)"
+    using not_occurs var_2_sred by blast
+  ultimately have "((Unit, Susp pi X) # xs, ys) \<turnstile> s2 \<bullet> [(X, swap (rev pi) Unit)] \<leadsto>\<^sup>* P2"
+    using sred_rtc_step by simp
+  then show "\<exists>s1. ((Unit, Susp pi X) # xs, ys) \<turnstile> s1 \<leadsto>\<^sup>* P2" 
+    by auto
+next
+  case ("8_3" a pi X xs ys nabla s)
+  hence "sred_fun
+     (apply_subst [(X, swap (rev pi) (Atom a))] (xs, ys), nabla, [(X, swap (rev pi) (Atom a))] \<bullet> s,
+      True) =
+    (P2, nabla', s', B)" by simp
+  moreover have not_occurs: "\<not> occurs X (Atom a)" by simp
+  ultimately obtain s2 where
+    more: "apply_subst [(X, swap (rev pi) (Atom a))] (xs, ys) \<turnstile> s2 \<leadsto>\<^sup>* P2"
+    using "8_3"(1) by auto
+  moreover have first: "((Atom a, Susp pi X) # xs, ys) \<turnstile> [(X, swap (rev pi) (Atom a))]
+      \<leadsto> apply_subst [(X, swap (rev pi) (Atom a))] (xs, ys)"
+    using not_occurs var_2_sred by blast
+  ultimately have "((Atom a, Susp pi X) # xs, ys) \<turnstile> s2 \<bullet> [(X, swap (rev pi) (Atom a))] \<leadsto>\<^sup>* P2"
+    using sred_rtc_step by simp
+  then show "\<exists>s1. ((Atom a, Susp pi X) # xs, ys) \<turnstile> s1 \<leadsto>\<^sup>* P2" 
+    by auto
+next
+  case ("8_4" t1 t2 pi X xs ys nabla s)
+  then show "\<exists>s1. ((Paar t1 t2, Susp pi X) # xs, ys) \<turnstile> s1 \<leadsto>\<^sup>* P2"
+  proof(cases "occurs X (Paar t1 t2)")
+    case True
+    hence "sred_fun (((Paar t1 t2, Susp pi X) # xs, ys), nabla, s, True) 
+      = (((Paar t1 t2, Susp pi X) # xs, ys), nabla, s, False)" by simp
+    with "8_4"(2) have "((Paar t1 t2, Susp pi X) # xs, ys) \<turnstile> [] \<leadsto>\<^sup>* P2" 
+      by auto
+    then show "\<exists>s1. ((Paar t1 t2, Susp pi X) # xs, ys) \<turnstile> s1 \<leadsto>\<^sup>* P2" 
+      by auto
+  next
+    case False
+    with "8_4"(2) have "sred_fun
+     (apply_subst [(X, swap (rev pi) (Paar t1 t2))] (xs, ys), nabla,
+      [(X, swap (rev pi) (Paar t1 t2))] \<bullet> s, True) =
+    (P2, nabla', s', B)" by simp
+    with "8_4"(1) False obtain s2 where
+    more: "apply_subst [(X, swap (rev pi) (Paar t1 t2))] (xs, ys) \<turnstile> s2 \<leadsto>\<^sup>* P2"
+      by auto
+    moreover have first: "((Paar t1 t2, Susp pi X) # xs, ys) \<turnstile> 
+        [(X, swap (rev pi) (Paar t1 t2))] \<leadsto> apply_subst [(X, swap (rev pi) (Paar t1 t2))] (xs, ys)"
+      using False var_2_sred occurs.simps by force
+    ultimately have "((Paar t1 t2, Susp pi X) # xs, ys) \<turnstile> 
+              s2 \<bullet> [(X, swap (rev pi) (Paar t1 t2))] \<leadsto>\<^sup>* P2"
+      using sred_rtc_step by simp
+    then show "\<exists>s1. ((Paar t1 t2, Susp pi X) # xs, ys) \<turnstile> s1 \<leadsto>\<^sup>* P2" 
+      by auto
+  qed
+next
+  case ("8_5" F t pi X xs ys nabla s)
+  then show "\<exists>s1. ((Func F t, Susp pi X) # xs, ys) \<turnstile> s1 \<leadsto>\<^sup>* P2"
+  proof(cases "occurs X (Func F t)")
+    case True
+    hence "sred_fun (((Func F t, Susp pi X) # xs, ys), nabla, s, True) 
+      = (((Func F t, Susp pi X) # xs, ys), nabla, s, False)" by simp
+    with "8_5"(2) have "((Func F t, Susp pi X) # xs, ys) \<turnstile> [] \<leadsto>\<^sup>* P2" 
+      by auto
+    then show "\<exists>s1. ((Func F t, Susp pi X) # xs, ys) \<turnstile> s1 \<leadsto>\<^sup>* P2" 
+      by auto
+  next
+    case False
+    with "8_5"(2) have "sred_fun
+     (apply_subst [(X, swap (rev pi) (Func F t))] (xs, ys), nabla,
+      [(X, swap (rev pi) (Func F t))] \<bullet> s, True) =
+    (P2, nabla', s', B)" by simp
+    with "8_5"(1) False obtain s2 where
+    more: "apply_subst [(X, swap (rev pi) (Func F t))] (xs, ys) \<turnstile> s2 \<leadsto>\<^sup>* P2"
+      by auto
+    moreover have first: "((Func F t, Susp pi X) # xs, ys) \<turnstile> 
+        [(X, swap (rev pi) (Func F t))] \<leadsto> apply_subst [(X, swap (rev pi) (Func F t))] (xs, ys)"
+      using False var_2_sred occurs.simps by force
+    ultimately have "((Func F t, Susp pi X) # xs, ys) \<turnstile> 
+              s2 \<bullet> [(X, swap (rev pi) (Func F t))] \<leadsto>\<^sup>* P2"
+      using sred_rtc_step by simp
+    then show "\<exists>s1. ((Func F t, Susp pi X) # xs, ys) \<turnstile> s1 \<leadsto>\<^sup>* P2" 
+      by auto
+  qed
+qed (auto)
+
+lemma sred_fun_completeness: 
+  assumes "P1 \<turnstile> s \<leadsto>\<^sup>* P2" and "P1 \<noteq> P2"
+  shows "\<exists>s1 B. sred_fun (P1, nabla, s2, True) = (P2, nabla, s1, B) 
+         \<and> (nabla \<Turnstile> subst (s \<bullet> s2) \<approx> subst s1)"
+  using assms
+proof(cases rule: sred_rtc.cases[OF assms(1)])
+  case (1 P1)
+  then show ?thesis
+    using assms(2) by auto
+next
+  case (2 P1 s1 P2 s2 P3)
+  then show ?thesis sorry
 qed
 
-lemma sred_rtc_to_sred_fun:
-  assumes "P1 \<turnstile> s1 \<leadsto>\<^sup>* P2"
-  shows "sred_fun (P1, [], True) = (P2, s1, True)"
-  sorry 
 
-lemma sred_fun_to_sred_rtc:
-  assumes  "sred_fun (P1, [], True) = (P2, s1, True)"
-  shows "P1 \<turnstile> s1 \<leadsto>\<^sup>* P2"
-  sorry
+
+
+function (sequential) cred_fun:: "(problem_type \<times> fresh_envs \<times> substs \<times> bool) \<Rightarrow> (problem_type \<times> fresh_envs \<times> substs \<times> bool)" 
+  where
+"cred_fun ((xs, (a \<sharp>? Unit)#ys), nabla, s, B) = cred_fun ((xs, ys), nabla, s, B)" |
+"cred_fun ((xs, (a \<sharp>? Paar t1 t2)#ys), nabla, s, B) = cred_fun ((xs, (a\<sharp>?t1)#(a\<sharp>?t2)#ys), nabla, s, B)" |
+"cred_fun ((xs, (a \<sharp>? Func F t)#ys), nabla, s, B) = cred_fun ((xs, (a\<sharp>?t)#ys), nabla, s, B)" |
+"cred_fun ((xs, (a \<sharp>? Abst b t)#ys), nabla, s, B) = (if a = b then
+                                                      cred_fun ((xs, ys), nabla, s, B)
+                                                    else
+                                                      cred_fun ((xs, (a\<sharp>?t)#ys), nabla, s, B))" |
+"cred_fun ((xs, (a \<sharp>? Atom b)#ys), nabla, s, B) = (if a = b then
+                                                      ((xs, (a \<sharp>? Atom a)#ys), nabla, s, False)
+                                                    else
+                                                      cred_fun ((xs, ys), nabla, s, B))" |
+"cred_fun ((xs, (a \<sharp>? Susp pi X)#ys), nabla, s, B) = cred_fun ((xs, ys), {((swapas (rev pi) a),X)}\<union>nabla, s, B)" |
+"cred_fun ((xs, []), nabla, s, B) = ((xs, []), nabla, s, B)"
+  by pat_completeness auto
+
+termination
+  apply(relation rank_sred)
+unfolding rank_sred_def by auto
+ 
 
 (*show these lemmas
 
 next steps:
-0. add nabla in the sred_fun 
-1. define the function for freshness (cred_fun)
-2. prove termination
+0. add nabla in the sred_fun (DONE)
+1. define the function for freshness (cred_fun) (DONE)
+2. prove termination (DONE)
 3. prove equivalence
 4. define the unif computable function that takes as input a problem and calls the functions
 sred_fun and cred_fun
